formal/SSBX/Foundation/Core/Attention.lean
@@ -11,8 +11,6 @@ Claim formalized here:
 -/
 import SSBX.Foundation.Core.HumanAlignment
 
-set_option maxRecDepth 1024
-
 namespace SSBX.Foundation.Core.Attention
 
 open SSBX.Roster
