formal/SSBX/Foundation/Core/ShengshengBuxi.lean
@@ -12,8 +12,6 @@ import SSBX.Core
 import SSBX.Roster
 import SSBX.Foundation.Core.MonadRoot
 
-set_option maxRecDepth 1024
-
 namespace SSBX.Foundation.Core.ShengshengBuxi
 
 open SSBX.Core.GammaProcess
